\begin{description}
    \item[Binomische Formeln] \
    \begin{itemize}
        \item[1.] $(a+b)^2=a^2+2ab+b^2$
        \item[2.] $(a-b)^2=a^2-2ab+b^2$
        \item[3.] $(a-b)(a+b)=a^2-b^2$
    \end{itemize}
    \item[Summenformel] \
    \begin{itemize}
        \item $(1-x)(1+x+x^2+\dots +x^n)=1-x^{n+1}$
        \item $(x-1)(1+x+x^2+\dots +x^n)=x^{n+1}-1$
    \end{itemize}
    \item[Distributivgesetze] \
    \begin{itemize}
        \item $a(a+b)=ab+ac$
        \item $(a+b)(c+d) = ac +ad + bc +bd$
    \end{itemize}
    \item[Vieta] $(x-a)(x-b) = x^2 - (a+b)x+ab$
    \item[Wurzel aus Nenner] $\frac{1}{\sqrt{2}}=\frac{\sqrt{2}}{2}$
    $$\frac{2+\sqrt{3}}{2-\sqrt{3}}=\frac{2+\sqrt{3}}{2-\sqrt{3}} \cdot \frac{2+\sqrt{3}}{2+\sqrt{3}}=\frac{4+4\sqrt{3}+3}{4-3}=7+4\sqrt{3}$$
\end{description}